% -*- compile-command: "latexmk -pdf document.tex" -*-
\documentclass{article}

\author{Sam Price}
\title{Orthogonal Matrix}

\newif\ifprinted%
\printedtrue%
\input{preamble}

\begin{document}

\maketitle

\begin{proposition}{}{}
  For any orthogonal matrix (matrix with columns forming an orthonormal basis) $M$,
  \[ M\inv = M^{T}. \]
\end{proposition}
\begin{proof}
  Let $M = [ v_{1} \cdots v_{n} ]$.
  We note that
  \[ (M^{T}M)_{ij} = v_{i} \cdot v_{j} = \abs{v_{i}}\abs{v_{j}}\cos\theta = \cos\theta. \]
  Where we can eliminate the scaling factor since $\abs{v_{k}} = 1$.
  Further, the $\cos\theta$ simply reduces to $\delta_{ij}$ due to the orthogonal nature of these vectors.
  So, we end with $(M^{T}M)_{ij} = (I_{n})_{ij} = \delta_{ij}$ and $M^{T}M = I_{n}$.

  We also know that $M$ must be invertible since it has full rank (we have a basis, after all)
  and so $(M^{T}M)M\inv = M\inv$ by above. However, we also then know $M^{T}(MM\inv) = M^{T}$.
  So, $M^{T} = M\inv$.
\end{proof}


\end{document}
