% -*- compile-command: "latexmk -pdf document.tex" -*-
\documentclass{article}

\author{Sam Price}
\title{Verify Pullback Properties}

\newif\ifprinted%
\printedtrue%
\input{preamble}

\begin{document}

\maketitle

Let $A, B, C$ be open in $\RR[n]$.
Then, let $\omega, \eta \in \Omega^{k}(C)$ and $\theta \in \Omega^{l}(C)$ with
\[ \alpha \from A \to \RR[n] \]
and
\[ \beta \from B \to \RR[n] \]
so that
\[ \alpha(A) \subset B, \beta(B) \subset C. \]

Verify:
\begin{enumerate}[start=1,label={\arabic*\rparen}]
  \item $\beta^{*}(a\omega + b\eta) = a\beta^{*}\omega + b\beta^{*}\eta$ for $a, b \in \RR$.
  \item $\beta^{*}(\omega \wedge \theta) = \beta^{*}\omega \wedge \beta^{*}\theta$.
  \item $(\beta \circ \alpha)^{*}\omega = \alpha^{*}(\beta^{*}\omega)$
\end{enumerate}

For the first, we simply have:
\begin{align*}
  \beta^{*}(a\omega + b\eta)(v_{1}, \ldots, v_{k}) &= (a\omega + b\eta)(\beta_{*}v_{1}, \ldots, \beta_{*}v_{k})\\
  &= (a\omega)(\beta_{*}v_{1}, \ldots, \beta_{*}v_{k}) + (b\eta)(\beta_{*}v_{1}, \ldots, \beta_{*}v_{k})\\
  &= a\beta^{*}\omega + b\beta^{*}\eta.
\end{align*}

The jump can happen because $k$-forms are linear themselves, which is quite nice.

The third is also simpler, since it is just function composition:
\begin{align*}
  (\beta \circ \alpha)^{*}\omega &= \omega(\beta \circ \alpha)_{*}\\
  &= \omega \circ (\beta_{*} \circ \alpha_{*}) \qquad \text{ from the book Lemma 29.1}\\
  &= (\omega \circ \beta_{*}) \circ \alpha_{*}\\
  &= \alpha^{*}(\omega \circ \beta_{*}) = \alpha^{*}(\beta^{*}\omega).
\end{align*}

The second is the last one I did, so I'll continue in this order.
\begin{align*}
  \beta^{*}(\omega \wedge \theta)(v_{1}, \ldots, v_{k + l}) &= (\omega \wedge \theta)(\beta_{*}v_{1}, \ldots, \beta_{*}v_{k + l})\\
  &= \omega(\beta_{*}v_{1}, \ldots, \beta_{*}v_{k}) \wedge \theta(\beta_{*}v_{k + 1}, \ldots, \beta_{*}v_{k + l})\\
  &= \beta^{*}\omega \wedge \beta^{*}\theta.
\end{align*}

\end{document}
