% -*- compile-command: "latexmk -pdf document.tex" -*-
\documentclass{article}

\author{Sam Price}
\title{Chapter 6, Section 30, Ex. 2}

\newif\ifprinted%
\printedtrue%
\input{preamble}

\begin{document}

\maketitle

Let $\omega = xy \,dx + 3 \,dy - yz \,dz$ and $\eta = x \,dx - yz^{2}\,dy + 2x \,dz$.
Verify
\begin{itemize}
  \item $d(d\omega) = 0$, and
  \item $d(\omega \wedge \eta) = d\omega \wedge \eta - \omega \wedge d\eta$.
\end{itemize}

For the first, let us calculate $d\omega$ first:
\begin{align*}
  d\omega &= (y\, dx + 0) \wedge dx\\
  &+ (x\, dx + 0 - z\, dz) \wedge dy\\
  &+ (0 - y\, dz) \wedge dz\\
  &= x\, dx \wedge dy + z\, dy \wedge dz.
\end{align*}
This is zero after another round of $d$ since the partials of $x$ and $z$
both vanish due to duplicated forms.

Now, we calculate different parts of the equation for the second step:
\[ d\eta = -2\,dx \wedge dz - 2yz\,dy\wedge dz. \]
\[ d\omega \wedge \eta = (2x^{2} + xz)\, dx\wedge dy\wedge dz. \]
\[ \omega \wedge d\eta = (6 - 2xy^{2}z)\,dx\wedge dy\wedge dz. \]
Subtracting, we find that
\begin{equation}\label{subtr}
  d\omega \wedge n - \omega \wedge d\eta = (2x^{2} + xz - 6 + 2xy^{2}z) \, dx\wedge dy\wedge dz.
\end{equation}

Looking to the left hand side, we see that
\[
  \omega \wedge \eta = (-xy^{2}z^{2} - 3x) \, dx \wedge dy
  + (2x^{2}y + xyz) \, dx \wedge dz
  + (6x - y^{2}z^{3}) \, dy\wedge dz.
\]
Taking the exterior derivative, we get
\[ d(\omega \wedge \eta) = (6 - 2x^{2} - xz - 2xy^{2}z) \, dx\wedge dy\wedge dz. \]

However, this is the \emph{negative} of~\eqref{subtr}.
Is this an issue with $(-1)^{3}$ being negative? I am lost.

\end{document}
