% -*- compile-command: "latexmk -pdf document.tex" -*-
\documentclass{article}

\author{Sam Price}
\title{Derivative Properties}

\newif\ifprinted%
\printedtrue%
\input{preamble}

\begin{document}

\maketitle

\begin{proposition}{}{}
  The derivative $D$ is linear.
  That is, for $f, g \from \RR[m] \to \RR[n]$ differentiable at $a \in \RR[m]$:
  \begin{enumerate}[start=1,label={(\alph*)}]
    \item $D(f + g) = Df + Dg$, and
    \item $D(\lambda f) = \lambda Df$.
  \end{enumerate}
\end{proposition}
\begin{proof}
  We show this by first ``assuming'' the derivative is correct, and then showing it does satisfy the property the (unique) matrix should.
  First, we see that for $f + g$:
  \begin{align*}
    \frac{(f + g)(a + h) - (f + g)(a) - (Df + Dg) \cdot h}{\abs{h}} &= \frac{f(a + h) - f(a) - (Df)h + g(a + h) - g(a) - (Dg)h}{\abs{h}}\\
    &= \frac{f(a + h) - f(a) - Df h}{\abs{h}} + \frac{g(a + h) - g(a) - Dg h}{\abs{h}} \to 0 + 0 = 0.
  \end{align*}
  Nearly identically for some $\lambda \in \RR$:
  \[
    \frac{(\lambda f)(a + h) - (\lambda f)(a) - (\lambda Df)h}{\abs{h}} = \lambda\frac{f(a + h) - f(a) - Df h}{\abs{h}} \to \lambda \cdot 0 = 0.
  \]
\end{proof}


\end{document}
